comment追加

main.ml
@@ -11,7 +11,7 @@ let mem = {
   nodes  = nodes;
   frees  = [];
   marker = (fun _ -> Unmarked);
-  pointer = (assoc [("a", "e"); ("e", "d")])
+  next = (assoc [("a", "e"); ("e", "d")])
 }
 
 let dec x y = x = y;;
@@ -23,7 +23,7 @@ let of_marker = function
     Marked -> "M"
   | Unmarked -> " "
 
-let of_pointer = function
+let of_next = function
     Some n -> Printf.sprintf "-> %s" n
   | None -> ""
 
@@ -31,7 +31,7 @@ let show { roots  = roots;
 	   nodes  = nodes;
 	   frees  = frees;
 	   marker = marker;
-	   pointer = pointer; } =
+	   next = next; } =
   Printf.sprintf "ROOTS: %s\nFREES: %s\nNODES:\n%s"
     (of_list roots)
     (of_list frees)
@@ -39,14 +39,14 @@ let show { roots  = roots;
 				     Printf.sprintf "%s %s %s"
 				       (of_marker  (marker n))
 				       n
-				       (of_pointer (pointer n)))
+				       (of_next (next n)))
 			   nodes))
 let _ =
   print_endline "=== init ===";
   print_endline (show mem);
   print_endline "";
   print_endline "=== mark ===";
-  print_endline (show (markerPhase dec mem));
+  print_endline (show (mark_phase dec mem));
   print_endline "";
   print_endline "=== sweep ===";
   print_endline (show (gc dec mem));
